replace barrett_reduction with almost_montgomery_reduction

code/ed25519/Hacl.Impl.Ed25519.PointEqual.fst
@@ -11,43 +11,11 @@ open Lib.Buffer
 open Hacl.Bignum25519
 
 module F51 = Hacl.Impl.Ed25519.Field51
-module F56 = Hacl.Impl.BignumQ.Mul
 module S51 = Hacl.Spec.Curve25519.Field51.Definition
 
 module SC = Spec.Curve25519
 
 #reset-options "--z3rlimit 20 --max_fuel 0 --max_ifuel 0"
-
-val gte_q:
-  s:lbuffer uint64 5ul ->
-  Stack bool
-    (requires fun h -> live h s /\
-      F56.qelem_fits h s (1, 1, 1, 1, 1)
-     )
-    (ensures  fun h0 b h1 -> h0 == h1 /\
-      (b <==> F56.as_nat h0 s >= Spec.Ed25519.q)
-    )
-
-[@CInline]
-let gte_q s =
-  let h0 = ST.get() in
-  let s0 = s.(0ul) in
-  let s1 = s.(1ul) in
-  let s2 = s.(2ul) in
-  let s3 = s.(3ul) in
-  let s4 = s.(4ul) in
-  assert_norm (Spec.Ed25519.q == 0x1000000000000000000000000000000014def9dea2f79cd65812631a5cf5d3ed);
-  let open FStar.UInt64 in
-  let open Lib.RawIntTypes in
-  if u64_to_UInt64 s4 >^ 0x00000010000000uL then true
-  else if u64_to_UInt64 s4 <^ 0x00000010000000uL then false
-  else (if u64_to_UInt64 s3 >^ 0x00000000000000uL then true
-  else if u64_to_UInt64 s2 >^ 0x000000000014deuL then true
-  else if u64_to_UInt64 s2 <^ 0x000000000014deuL then false
-  else if u64_to_UInt64 s1 >^ 0xf9dea2f79cd658uL then true
-  else if u64_to_UInt64 s1 <^ 0xf9dea2f79cd658uL then false
-  else if u64_to_UInt64 s0 >=^ 0x12631a5cf5d3eduL then true
-  else false)
 
 let u51 = n:nat{n < 0x8000000000000}
 
