code/ed25519/Hacl.Impl.BignumQ.fst
@@ -1,0 +1,165 @@
+module Hacl.Impl.BignumQ
+
+module ST = FStar.HyperStack.ST
+open FStar.HyperStack
+open FStar.HyperStack.All
+open FStar.Mul
+
+open Lib.IntTypes
+open Lib.Buffer
+
+module BSeq = Lib.ByteSequence
+module BD = Hacl.Bignum.Definitions
+module BN = Hacl.Bignum
+module AM = Hacl.Bignum.AlmostMontgomery
+module BR = Hacl.Bignum.ModReduction
+
+module SD = Hacl.Spec.Bignum.Definitions
+module SN = Hacl.Spec.Bignum
+
+friend Hacl.Bignum256
+
+#set-options "--z3rlimit 50 --fuel 0 --ifuel 0"
+
+inline_for_extraction noextract
+instance km: AM.almost_mont U64 =
+  Hacl.Bignum256.almost_mont_inst
+
+
+inline_for_extraction noextract
+val make_u64_4 (out:lbuffer uint64 4ul) (f0 f1 f2 f3:uint64) : Stack unit
+  (requires fun h -> live h out)
+  (ensures  fun h0 _ h1 -> modifies (loc out) h0 h1 /\
+    BD.bn_v #_ #4ul h1 out == v f0 + v f1 * pow2 64 + v f2 * pow2 128 + v f3 * pow2 192)
+
+let make_u64_4 out f0 f1 f2 f3 =
+  out.(0ul) <- f0;
+  out.(1ul) <- f1;
+  out.(2ul) <- f2;
+  out.(3ul) <- f3;
+  let h = ST.get () in
+  SD.bn_eval_unfold_i (as_seq h out) 4;
+  SD.bn_eval_unfold_i (as_seq h out) 3;
+  SD.bn_eval_unfold_i (as_seq h out) 2;
+  SD.bn_eval_unfold_i (as_seq h out) 1;
+  SD.bn_eval0 (as_seq h out)
+
+
+inline_for_extraction noextract
+val make_q: q:lbuffer uint64 4ul -> Stack unit
+  (requires fun h -> live h q)
+  (ensures  fun h0 _ h1 -> modifies (loc q) h0 h1 /\
+    BD.bn_v h1 q == Spec.Ed25519.q)
+
+let make_q q =
+  [@inline_let] let (f0, f1, f2, f3) =
+   (u64 0x5812631a5cf5d3ed,
+    u64 0x14def9dea2f79cd6,
+    u64 0x0,
+    u64 0x1000000000000000) in
+
+  make_u64_4 q f0 f1 f2 f3;
+  assert_norm (Spec.Ed25519.q == v f0 + v f1 * pow2 64 + v f2 * pow2 128 + v f3 * pow2 192)
+
+
+inline_for_extraction noextract
+val make_mu: unit -> mu:uint64{(1 + Spec.Ed25519.q * v mu) % pow2 64 == 0}
+let make_mu () =
+  [@inline_let] let mu = u64 0xd2b51da312547e1b in
+  assert_norm ((1 + Spec.Ed25519.q * v mu) % pow2 64 = 0);
+  mu
+
+
+inline_for_extraction noextract
+val make_r2_modq: r2:lbuffer uint64 4ul -> Stack unit
+  (requires fun h -> live h r2)
+  (ensures  fun h0 _ h1 -> modifies (loc r2) h0 h1 /\
+    BD.bn_v h1 r2 == pow2 512 % Spec.Ed25519.q)
+
+let make_r2_modq r2 =
+  [@inline_let] let (f0, f1, f2, f3) =
+   (u64 0xa40611e3449c0f01,
+    u64 0xd00e1ba768859347,
+    u64 0xceec73d217f5be65,
+    u64 0x399411b7c309a3d) in
+
+  make_u64_4 r2 f0 f1 f2 f3;
+  assert_norm (pow2 512 % Spec.Ed25519.q ==
+    v f0 + v f1 * pow2 64 + v f2 * pow2 128 + v f3 * pow2 192)
+
+
+[@CInline]
+let modq a res =
+  push_frame ();
+  let q = create 4ul (u64 0) in
+  make_q q;
+  assert_norm (Spec.Ed25519.q % 2 = 1);
+  assert_norm (pow2 252 < Spec.Ed25519.q);
+
+  [@inline_let] let mu = make_mu () in
+  let r2 = create 4ul (u64 0) in
+  make_r2_modq r2;
+  BR.bn_mod_slow_precomp km q mu r2 a res;
+  pop_frame ()
+
+
+val lemma_mul_lt: a:nat -> b:nat -> c:nat -> d:nat -> Lemma
+  (requires a < c /\ b < d)
+  (ensures  a * b < c * d)
+
+let lemma_mul_lt a b c d = ()
+
+
+[@CInline]
+let mul_add_modq a b c res =
+  push_frame ();
+  let tmp = create 8ul (u64 0) in
+  // mul4 a b tmp;
+  km.AM.bn.BN.mul a b tmp;
+  let h0 = ST.get () in
+  SN.bn_mul_lemma (as_seq h0 a) (as_seq h0 b);
+  assert (BD.bn_v h0 tmp == BD.bn_v h0 a * BD.bn_v h0 b);
+
+  SD.bn_eval_bound (as_seq h0 b) 4;
+  lemma_mul_lt (BD.bn_v h0 a) (BD.bn_v h0 b) Spec.Ed25519.q (pow2 256);
+  assert_norm (Spec.Ed25519.q + Spec.Ed25519.q * pow2 256 < pow2 512);
+
+  let c1 = BN.bn_add 8ul tmp 4ul c tmp in
+  let h1 = ST.get () in
+  SN.bn_add_lemma (as_seq h0 tmp) (as_seq h0 c);
+  assert (BD.bn_v h1 tmp + v c1 * pow2 512 == BD.bn_v h0 tmp + BD.bn_v h0 c);
+  SD.bn_eval_bound (as_seq h1 tmp) 8;
+  assert (v c1 = 0);
+  modq tmp res;
+  Math.Lemmas.lemma_mod_plus_distr_r
+    (BD.bn_v h0 c) (BD.bn_v h0 a * BD.bn_v h0 b) Spec.Ed25519.q;
+  pop_frame ()
+
+
+[@CInline]
+let gte_q s =
+  // TODO: add _vartime version?
+  push_frame ();
+  let q = create 4ul (u64 0) in
+  make_q q;
+
+  let b = BN.bn_lt_mask 4ul s q in
+  let h = ST.get () in
+  SN.bn_lt_mask_lemma (as_seq h s) (as_seq h q);
+  assert (if v b = 0 then BD.bn_v h s >= BD.bn_v h q else BD.bn_v h s < BD.bn_v h q);
+  pop_frame ();
+  Hacl.Spec.Bignum.Base.unsafe_bool_of_limb0 b
+
+
+[@CInline]
+let load_32_bytes out b =
+  let h0 = ST.get () in
+  Hacl.Bignum.Convert.mk_bn_from_bytes_le true 32ul b out;
+  Hacl.Spec.Bignum.Convert.bn_from_bytes_le_lemma #U64 32 (as_seq h0 b)
+
+
+[@CInline]
+let store_32_bytes out b =
+  let h0 = ST.get () in
+  Hacl.Bignum.Convert.mk_bn_to_bytes_le true 32ul b out;
+  Hacl.Spec.Bignum.Convert.bn_to_bytes_le_lemma 32 (as_seq h0 b)
