code/ed25519/Hacl.Impl.BignumQ.fsti
@@ -1,0 +1,62 @@
+module Hacl.Impl.BignumQ
+
+module ST = FStar.HyperStack.ST
+open FStar.HyperStack
+open FStar.HyperStack.All
+open FStar.Mul
+
+open Lib.IntTypes
+open Lib.Buffer
+
+module BSeq = Lib.ByteSequence
+module BD = Hacl.Bignum.Definitions
+
+#set-options "--z3rlimit 50 --fuel 0 --ifuel 0"
+
+val modq: a:lbuffer uint64 8ul -> res:lbuffer uint64 4ul -> Stack unit
+  (requires fun h ->
+    live h a /\ live h res /\ disjoint a res)
+  (ensures  fun h0 _ h1 -> modifies (loc res) h0 h1 /\
+    BD.bn_v h1 res == BD.bn_v h0 a % Spec.Ed25519.q)
+
+
+val mul_add_modq:
+    a:lbuffer uint64 4ul
+  -> b:lbuffer uint64 4ul
+  -> c:lbuffer uint64 4ul
+  -> res:lbuffer uint64 4ul ->
+  Stack unit
+  (requires fun h ->
+    live h a /\ live h b /\ live h c /\ live h res /\
+    eq_or_disjoint a b /\
+    eq_or_disjoint res a /\ eq_or_disjoint res b /\ eq_or_disjoint res c /\
+    BD.bn_v h a < Spec.Ed25519.q /\ BD.bn_v h c < Spec.Ed25519.q)
+  (ensures  fun h0 _ h1 -> modifies (loc res) h0 h1 /\
+    BD.bn_v h1 res ==
+    (BD.bn_v h0 c + (BD.bn_v h0 a * BD.bn_v h0 b % Spec.Ed25519.q)) % Spec.Ed25519.q)
+
+
+val gte_q: s:lbuffer uint64 4ul -> Stack bool
+  (requires fun h -> live h s)
+  (ensures  fun h0 b h1 -> modifies0 h0 h1 /\
+    (b <==> BD.bn_v h0 s >= Spec.Ed25519.q))
+
+
+val load_32_bytes:
+  out:lbuffer uint64 4ul
+  -> b:lbuffer uint8 32ul ->
+  Stack unit
+  (requires fun h -> live h out /\ live h b /\ disjoint out b)
+  (ensures  fun h0 _ h1 -> modifies (loc out) h0 h1 /\
+    BD.bn_v h1 out == BSeq.nat_from_bytes_le (as_seq h0 b))
+
+
+val store_32_bytes:
+    out:lbuffer uint8 32ul
+  -> b:lbuffer uint64 4ul ->
+  Stack unit
+  (requires fun h ->
+    live h out /\ live h b /\ disjoint out b /\
+    BD.bn_v h b < Spec.Ed25519.q)
+  (ensures  fun h0 _ h1 -> modifies (loc out) h0 h1 /\
+    as_seq h1 out == BSeq.nat_to_bytes_le 32 (BD.bn_v h0 b))
