Makefile
@@ -674,7 +674,8 @@ INTRINSIC_INT_FLAGS = \
   -add-include 'Hacl_P256:"lib_intrinsics.h"' \
   -add-include 'Hacl_Bignum:"lib_intrinsics.h"' \
   -add-include 'Hacl_Bignum_Base:"lib_intrinsics.h"' \
-  -add-include 'Hacl_K256_ECDSA:"lib_intrinsics.h"'
+  -add-include 'Hacl_K256_ECDSA:"lib_intrinsics.h"' \
+  -add-include 'Hacl_Ed25519:"lib_intrinsics.h"'
 
 # Disables tests; overriden in Wasm where tests indicate what can be compiled.
 TEST_FLAGS = -bundle Test,Test.*,Hacl.Test.*
